
---

- In electrodynamics, one frequently encounters problems involving two points—typically, 
  - a source point, $\mathbf{r}'$, where an electric charge is located, 
  - and a field point, $\mathbf{r}$, at which you are calculating the electric or magnetic field. 

- It pays to adopt right from the start some short-hand notation for the separation vector from the source point to the field point. 
- I shall use for this purpose the script letter $\vec{\gamma}$:  

$$
\vec{\gamma} \equiv \mathbf{r} - \mathbf{r}'
$$

- Its magnitude is  

$$
\gamma = |\mathbf{r} - \mathbf{r}'|
$$

- and a unit vector 
  - in the direction from $\mathbf{r}'$ to $\mathbf{r}$ is  
$$
\hat{\gamma} = \frac{\vec{\gamma}}{\gamma} = \frac{\mathbf{r} - \mathbf{r}'}{|\mathbf{r} - \mathbf{r}'|}
$$

- In Cartesian coordinates,  
$$
\vec{\gamma} = (x - x')\hat{\mathbf{x}} + (y - y')\hat{\mathbf{y}} + (z - z')\hat{\mathbf{z}}
$$

$$
\gamma = \sqrt{(x - x')^2 + (y - y')^2 + (z - z')^2}
$$

$$
\hat{\gamma} = \frac{(x - x')\hat{\mathbf{x}} + (y - y')\hat{\mathbf{y}} + (z - z')\hat{\mathbf{z}}}{\sqrt{(x - x')^2 + (y - y')^2 + (z - z')^2}}
$$

(from which you can appreciate the economy of the script-$\mathscr{r}$ notation).  

---

- 間隔向量，$\vec{\gamma} = \mathbf{r}-\mathbf{r}'$ ，
  - 代表source point指向field point的向量
- 每一本電磁學都是這麼表示，
  - r，代表場的位置，
  - r一撇，代表電荷的位置。
- 但是，只有Griffiths使用了一個特殊的符號代表間隔向量
- 那個符號很難打出來，按照Griffiths自己的備註，
  - 使用的是 "Kaufmann" 字體，
  - 但這個字體在 TeX 中非常難以安裝。
  - TeX 使用者可以從Griffiths的網站下載一個相當不錯的相似版本。
- 我這邊直接用 $\gamma$ 表示

---

### 習題1-13

$$
\nabla\gamma = \nabla\sqrt{(x - x')^2 + (y - y')^2 + (z - z')^2}
$$

$$
\nabla\gamma =
\frac{\partial \gamma}{\partial x} \,\hat{\mathbf{x}} +
\frac{\partial \gamma}{\partial y} \,\hat{\mathbf{y}} +
\frac{\partial \gamma}{\partial z} \,\hat{\mathbf{z}} 
$$

$$
\frac{\partial \gamma}{\partial x} = \frac{1}{2} \cdot \frac{2(x - x')}{\sqrt{(x - x')^2 + (y - y')^2 + (z - z')^2}} 
$$

$$
= \frac{x - x'}{\sqrt{(x - x')^2 + (y - y')^2 + (z - z')^2}}
= \frac{x - x'}{\gamma}
$$

Similarly,  

$$
\frac{\partial \gamma}{\partial y} = 
\frac{y - y'}{\gamma}
\quad
\frac{\partial \gamma}{\partial z} = 
\frac{z - z'}{\gamma}
$$

Thus,
$$
\nabla \gamma =
\frac{x - x'}{\gamma} \hat{\mathbf{x}}+
\frac{y - y'}{\gamma} \hat{\mathbf{y}}+
\frac{z - z'}{\gamma} \hat{\mathbf{z}}
$$

$$
= \frac{\vec{\gamma}}{\gamma} = \hat{\gamma}
$$

(a)
$$
\nabla(\gamma^2) = \nabla \left[{(x - x')^2 + (y - y')^2 + (z - z')^2} \right]
$$

$$
\nabla(\gamma^2) =
\frac{\partial (\gamma^2)}{\partial x} \,\hat{\mathbf{x}} +
\frac{\partial (\gamma^2)}{\partial y} \,\hat{\mathbf{y}} +
\frac{\partial (\gamma^2)}{\partial z} \,\hat{\mathbf{z}} 
$$

$$
\frac{\partial (\gamma^2)}{\partial x} = 2(x - x')
$$

Similarly,  

$$
\frac{\partial (\gamma^2)}{\partial y} = 2(y - y')
\quad
\frac{\partial (\gamma^2)}{\partial z} = 2(z - z')
$$

Thus,
$$
\nabla (\gamma^2) =
2(x - x') \hat{\mathbf{x}}+
2(y - y') \hat{\mathbf{y}}+
2(z - z') \hat{\mathbf{z}}
$$

$$
= 2\vec{\gamma}
$$

或者，透過連鎖律

$$
\nabla(\gamma^2) = 2\gamma\,\nabla(\gamma)
$$

$$
= 2\gamma\,\hat{\gamma} = 2\vec{\gamma}
$$

(b)
$$
\nabla \left( \frac{1}{\gamma} \right) = \frac{-1}{\gamma^2}\,\nabla(\gamma) = \frac{-\hat{\gamma}}{\gamma^2}
$$

(c)
$$
\nabla \left( \gamma^n \right) = n\gamma^{n-1}\,\nabla(\gamma) = n\gamma^{n-1} \, \hat{\gamma}
$$

---

### 對 source point 微分

$$
\nabla'\gamma = \nabla'\sqrt{(x - x')^2 + (y - y')^2 + (z - z')^2}
$$

$$
\nabla'\gamma =
\frac{\partial \gamma}{\partial x'} \,\hat{\mathbf{x}} +
\frac{\partial \gamma}{\partial y'} \,\hat{\mathbf{y}} +
\frac{\partial \gamma}{\partial z'} \,\hat{\mathbf{z}} 
$$

$$
\frac{\partial \gamma}{\partial x'} = \frac{1}{2} \cdot \frac{-2(x - x')}{\sqrt{(x - x')^2 + (y - y')^2 + (z - z')^2}} 
$$

$$
= \frac{-(x - x')}{\sqrt{(x - x')^2 + (y - y')^2 + (z - z')^2}}
= \frac{-(x - x')}{\gamma}
$$

Similarly,  

$$
\frac{\partial \gamma}{\partial y'} = 
\frac{-(y - y')}{\gamma}
\quad
\frac{\partial \gamma}{\partial z'} = 
\frac{-(z - z')}{\gamma}
$$

Thus,
$$
\nabla' \gamma =
\frac{-(x - x')}{\gamma} \hat{\mathbf{x}}+
\frac{-(y - y')}{\gamma} \hat{\mathbf{y}}+
\frac{-(z - z')}{\gamma} \hat{\mathbf{z}}
$$

$$
= \frac{-\vec{\gamma}}{\gamma} = -\hat{\gamma}
$$

$$
\nabla' \left( \frac{1}{\gamma} \right) = \frac{-1}{\gamma^2}\,\nabla'(\gamma) = \frac{\hat{\gamma}}{\gamma^2}
$$
