
**Example 3.3** 
 
- Two infinite grounded metal plates lie parallel to the $xz$-plane, one at $y = 0$, the other at $y = a$ (Fig. 3.17). 
- The left end, at $x = 0$, 
  - is closed off with an infinite strip 
  - insulated from the two plates 
  - and maintained at a specific potential $V_0(y)$. 
- Find the potential inside this “slot.”  

**Solution**  
- The configuration is independent of $z$, 
- so this is really a two-dimensional problem. 
- In mathematical terms, we must solve Laplace’s equation:
$$
\frac{\partial^2 V}{\partial x^2} + \frac{\partial^2 V}{\partial y^2} = 0
$$

- subject to the boundary conditions:  
(i) $V = 0$ when $y = 0$,  
(ii) $V = 0$ when $y = a$,  
(iii) $V = V_0(y)$ when $x = 0$,  
(iv) $V \to 0$ as $x \to \infty$.  

- (The latter, although not explicitly stated in the problem, 
  - is necessary on physical grounds: 
  - as you get farther and farther away from the “hot” strip at $x = 0$, 
  - the potential should drop to zero.) 
- Since the potential is specified on all boundaries, the answer is uniquely determined.  

- The first step is to look for solutions in the form of products:  
$$
V(x, y) = X(x) Y(y)
$$

- On the face of it, this is an absurd restriction—
  - the overwhelming majority of solutions to Laplace’s equation do not have such a form. 
  - For example, $V(x, y) = (5x + 6y)$ satisfies Laplace’s equation, but you can’t express it as the product of a function of $x$ times a function of $y$. 
- Obviously, we’re only going to get a tiny subset of all possible solutions by this means, 
- and it would be a miracle 
  - if one of them happened to fit the boundary conditions of our problem...  

- But hang on, because the solutions we do get are very special, 
- and it turns out that by pasting them together 
  - we can construct the general solution.  

- Anyway, substituting $V(x, y) = X(x) Y(y)$ into Laplace’s equation, we obtain:  
$$
Y \frac{d^2 X}{dx^2} + X \frac{d^2 Y}{dy^2} = 0
$$

- The next step is to “separate the variables” 
- (i.e., collect all the $x$-dependence into one term and all the $y$-dependence into another). 
- Typically, this is accomplished by dividing through by $V$:  
$$
\frac{1}{X} \frac{d^2 X}{dx^2} + \frac{1}{Y} \frac{d^2 Y}{dy^2} = 0
$$

- Here, the first term depends only on $x$ 
- and the second only on $y$; 
- in other words, we have an equation of the form  
$$
f(x) + g(y) = 0
$$

- Now, there’s only one way this could possibly be true: 
- $f(x)$ and $g(y)$ must both be constant. 
- For if $f(x)$ changed as you vary $x$, 
  - then if we held $y$ fixed and fiddled with $x$, 
  - the sum $f(x) + g(y)$ would change, 
  - in violation of the equation above, 
  - which states that it is always zero. 
  - (That’s a simple but somewhat elusive argument; 
  - don’t accept it without due thought, 
  - because the whole method rides on it.)  

- It follows that  
$$
\frac{1}{X} \frac{d^2 X}{dx^2} = C_1, \quad \frac{1}{Y} \frac{d^2 Y}{dy^2} = C_2
$$

- with  
$$
C_1 + C_2 = 0.
$$

- One of these constants is positive, the other negative (or perhaps both are zero). 
- In general, one must investigate all possibilities; 
- however, in our particular problem, 
  - we need $C_1$ positive 
  - and $C_2$ negative, 
  - for reasons that will appear in a moment.  

- Thus, we get the equations  
$$
\frac{d^2 X}{dx^2} = k^2 X, \quad \frac{d^2 Y}{dy^2} = -k^2 Y
$$

- Notice what has happened: A partial differential equation has been converted into two ordinary differential equations. 
- The advantage of this is obvious—ordinary differential equations are much easier to solve.  

- Indeed, the general solutions are  
$$
X(x) = A e^{kx} + B e^{-kx}
$$

$$
Y(y) = C \sin k y + D \cos k y
$$

- So, the potential takes the form  
$$
V(x, y) = (A e^{kx} + B e^{-kx}) (C \sin k y + D \cos k y)
$$

- This is the appropriate separable solution to Laplace’s equation; 
- it remains to impose the boundary conditions and determine the constants.  

- To begin at the end, condition (iv) requires that $A = 0$, 
  - so that $X(x)$ does not grow unbounded as $x \to \infty$. 
- Absorbing $B$ into $C$ and $D$, we are left with  
$$
V(x, y) = e^{-kx} (C \sin k y + D \cos k y)
$$

- Condition (i) now demands that $D = 0$, so  
$$
V(x, y) = C e^{-kx} \sin k y
$$

- Meanwhile, condition (ii) yields  
$$
\sin k a = 0,
$$

- from which it follows that  
$$
k = \frac{n \pi}{a}, \quad (n = 1, 2, 3, \dots)
$$

- (At this point, you can see why we chose $C_1$ positive and $C_2$ negative: 
- If $X(x)$ were sinusoidal, we could never arrange for it to go to zero at infinity, 
- and if $Y(y)$ were exponential, we could not make it vanish at both $y = 0$ and $y = a$. 
- Incidentally, $n = 0$ is no good, for in that case the potential vanishes everywhere. 
- Negative $n$ values are also excluded.)  

- That’s as far as we can go using separable solutions, 
- and unless $V_0(y)$ just happens to have the form $\sin (n\pi y/a)$ for some integer $n$, we simply can’t fit the final boundary condition at $x = 0$.  

- But now comes the crucial step that redeems the method: 
  - Separation of variables has given us an infinite family of solutions (one for each $n$), 
  - and whereas none of them by itself satisfies the final boundary condition, 
  - it is possible to combine them in a way that does.  

- Laplace’s equation is linear, meaning that if $V_1, V_2, V_3, \dots$ satisfy it, so does any linear combination:  
$$
V = \alpha_1 V_1 + \alpha_2 V_2 + \alpha_3 V_3 + \dots
$$

- Thus, we can construct a more general solution:  
$$
V(x, y) = \sum_{n=1}^{\infty} C_n e^{-n \pi x / a} \sin \left(\frac{n \pi y}{a} \right)
$$

- This still satisfies three of the boundary conditions; the question is whether we can choose the coefficients $C_n$ to fit the final boundary condition:  
$$
V(0, y) = \sum_{n=1}^{\infty} C_n \sin \left(\frac{n \pi y}{a} \right) = V_0(y)
$$

- This is just a Fourier sine series for $V_0(y)$, allowing us to determine $C_n$.

- Well, you may recognize this sum—
  - it’s a Fourier sine series. 
- And Dirichlet’s theorem guarantees that 
  - virtually any function $V_0(y)$—it can even have a finite number of discontinuities—
  - can be expanded in such a series. 
- But how do we actually determine the coefficients $C_n$, buried as they are in that infinite sum? 
- The device for accomplishing this is so lovely it deserves a name—
- I call it Fourier’s trick, though it seems Euler had used essentially the same idea somewhat earlier. 
- Here’s how it goes:

- Multiply
$$
V(0, y) = \sum_{n=1}^{\infty} C_n \sin \left(\frac{n \pi y}{a} \right) = V_0(y)
$$

- by $\sin(n' \pi y/a)$ 
  - (where $n'$ is a positive integer), 
  - and integrate from $0$ to $a$:
$$
\sum_{n=1}^{\infty} C_n \int_0^a \sin(n\pi y/a) \sin(n' \pi y/a) \, dy
$$

$$
= \int_0^a V_0(y) \sin(n' \pi y/a) \, dy
$$

- You can work out the integral on the left for yourself; the answer is
$$
\int_0^a \sin(n\pi y/a) \sin(n' \pi y/a) \, dy
$$

$$
=
\begin{cases}
0, & \text{if } n' \neq n, \\
a/2, & \text{if } n' = n.
\end{cases}
$$

- Thus, all the terms in the series drop out, 
  - save only the one where $n = n'$, and
    $$
    \sum_{n=1}^{\infty} C_n \int_0^a \sin(n\pi y/a) \sin(n' \pi y/a) \, dy
    $$ 
  - reduces to $(a/2) C_{n'}$. 
- Conclusion:
$$
C_n = \frac{2}{a} \int_0^a V_0(y) \sin(n\pi y/a) \, dy
$$

- That does it:
    $$
    V(x, y) = \sum_{n=1}^{\infty} C_n e^{-n \pi x / a} \sin \left(\frac{n \pi y}{a} \right)
    $$
    - is the solution
    - with coefficients given by
    $$
    C_n = \frac{2}{a} \int_0^a V_0(y) \sin(n\pi y/a) \, dy
    $$
    - subject to the boundary conditions:  
    (i) $V = 0$ when $y = 0$,  
    (ii) $V = 0$ when $y = a$,  
    (iii) $V = V_0(y)$ when $x = 0$,  
    (iv) $V \to 0$ as $x \to \infty$.  

---

- 先驗算一下，這樣的解釋否滿足拉普拉斯方程與邊界條件

1. **边界条件 (i) 和 (ii)：**  
   当 $y = 0$ 或 $y = a$ 时，正弦项 $\sin(n\pi y/a)$ 为零，因此级数中每一项均为零，总和 $V(x,0) = V(x,a) = 0$，满足条件。

2. **边界条件 (iv)：**  
   当 $x \to \infty$ 时，指数项 $e^{-n\pi x/a}$ 趋近于零。由于每一项被指数衰减控制且级数一致收敛，总和 $V(x,y) \to 0$，满足条件。

3. **边界条件 (iii)：**  
   当 $x = 0$ 时，解退化为傅里叶正弦级数：  
   $$
   V(0,y) = \sum_{n=1}^\infty C_n \sin(n\pi y/a),
   $$  
   其中系数 $C_n$ 通过正交性确定。将两边乘以 $\sin(m\pi y/a)$ 并在区间 \([0,a]\) 积分，利用正交关系：  
   $$
   \int_0^a \sin(n\pi y/a) \sin(m\pi y/a) dy = \frac{a}{2} \delta_{nm},
   $$  
   直接导出 $C_n = \frac{2}{a} \int_0^a V_0(y) \sin(n\pi y/a) dy$，从而确保 $V(0,y) = V_0(y)$。

4. **拉普拉斯方程验证：**  
   每一项 $C_n e^{-n\pi x/a} \sin(n\pi y/a)$ 均满足二维拉普拉斯方程：  
   $$
   \nabla^2 V = \frac{\partial^2 V}{\partial x^2} + \frac{\partial^2 V}{\partial y^2} = 0.
   $$  
   具体计算二阶导数后，

   每一项對x的二階導數，會是 $(\frac{n\pi}{a})^2 \times$原項

   每一项對y的二階導數，會是 $-(\frac{n\pi}{a})^2 \times$原項

   正负项相消，总和为零。级数解作为线性叠加，自然也满足方程。

综上，该解严格满足所有边界条件和控制方程，因此是问题的正确解。

**结论：**  
给定解 $V(x,y)$ 满足所有边界条件和拉普拉斯方程，系数 $C_n$ 的表达式通过傅里叶正弦展开的正交性确定，验证过程完整有效。

---

