

---

**Example 4.7.** 

- A sphere of homogeneous linear dielectric material is placed in an otherwise uniform electric field $\vec{E}_o$. 
- Find the electric field inside the sphere.

**Solution** 

- This is reminiscent of Example 3.8, in which an uncharged conducting sphere was introduced into a uniform field. 
- In that case, the field of the induced charge canceled $\vec{E}_o$ within the sphere; 
- in a dielectric, the cancellation (from the bound charge) is incomplete.
- Our problem is to solve Laplace’s equation for $V_{in}(r,θ)$ when $r \leq R$, and $V_{out}(r,θ)$ when $r \geq R$, subject to the boundary conditions:

1. $V_{\text{in}} = V_{\text{out}}, \quad \text{at } r = R$
2. $\epsilon_r \frac{\partial V_{\text{in}}}{\partial r} = \frac{\partial V_{\text{out}}}{\partial r}, \quad \text{at } r = R$
3. $V_{\text{out}} \to -E_0 r \cos\theta, \quad \text{for } r \to \infty$  

- (The second condition follows from Eq. 4.41, since there is no free charge at the surface.)

- Inside the sphere, Eq. 3.65 gives:
$$
V_{\text{in}}(r, \theta) = \sum_{l=0}^{\infty} A_l r^l P_l(\cos\theta)
$$

- Outside the sphere, considering condition (iii), we have:
$$
V_{\text{out}}(r, \theta) = -E_0 r \cos\theta + \sum_{l=0}^{\infty} \frac{B_l}{r^{l+1}} P_l(\cos\theta)
$$

- Boundary condition (i) requires:
$$
\sum_{l=0}^{\infty} A_l R^l P_l(\cos\theta)
$$

$$
= -E_0 R \cos\theta + \sum_{l=0}^{\infty} \frac{B_l}{R^{l+1}} P_l(\cos\theta)
$$

- which leads to:
$$
A_l R^l = \frac{B_l}{R^{l+1}} , \quad \text{for } l \neq 1  \quad (1)
$$

$$
A_1 R = -E_0 R + \frac{B_1}{R^2} \quad (2)
$$

- Meanwhile, condition (ii) yields:
$$
\epsilon_r \sum_{l=0}^{\infty} l A_l R^{l-1} P_l(\cos\theta)
$$

$$
= -E_0 \cos\theta - \sum_{l=0}^{\infty} \frac{(l+1) B_l}{R^{l+2} } P_l(\cos\theta)
$$

- which simplifies to:
$$
\epsilon_r l A_l R^{l-1} = -\frac{(l+1) B_l}{R^{l+2} }, \quad \text{for } l \neq 1  \quad (3) 
$$

$$
\epsilon_r A_1 = -E_0 - \frac{2B_1}{R^{3}}  \quad (4)      
$$

- It follows that $A_l = B_l = 0$ for $l \neq 1$, and:
$$
A_1 = \frac{-3}{\epsilon_r + 2} E_0
$$

$$
B_1 = \frac{\epsilon_r - 1}{\epsilon_r + 2} R^3 E_0
$$

- Thus, the potential inside the sphere is:
$$
V_{\text{in}}(r, \theta) = -\frac{3E_0}{\epsilon_r + 2} r \cos\theta = -\frac{3E_0}{\epsilon_r + 2} z
$$

- Hence, the electric field inside the sphere is (surprisingly) uniform:
$$
E = \frac{3}{\epsilon_r + 2} E_0
$$

---

### 前言

- 這和均勻極化球的差別在於，我們計算均勻極化球造成的電場時，沒有去管那顆均勻極化球的均勻極化向量是哪來的，在那邊那是給定條件。
- 而這裡，不是給定一個均勻極化球，而是給定一個線性均勻的電介質。
- 這個電介質會被極化，然後極化的電介質會影響電場，進一步影響極化，這是個無限的交互作用過程。
- 這沒辦法單靠理論計算，必須等到一個穩態階段，我們直接去測量，聯繫最終的總電場與極化向量場的關聯，他就是電極化率，或是等價的介電常數，介質的電容率，這其實是有點複雜的細節，
- 本科生電磁學不包括這些內容，而是會像本例題一樣，直接給定介電常數，讓你去做一些基本的計算。

### 解說

- 球座標系中的軸對稱問題，在無自由電荷的區域，滿足 Laplace 方程的標量場可用勒讓德級數展開
- 但這裡我們不進行完整的級數展開。
- 我們給定的邊界條件，總是會使得，勒讓德級數只剩有限項，甚至剩下一項。
- 這題中，解這個問題一開始就能夠知道，勒讓德級數大概只會剩下，$l=1$的那一項。
- 這還是要去確認的，但範例中，並未給出完整的確認過程，以下仔細檢視。
- 根據無限遠的邊界條件，就能猜出，只會剩下，$P_1(\cos\theta)$。
- 根據介電質球面兩側的邊界條件，當 $l\neq 1$
$$
A_l R^l = \frac{B_l}{R^{l+1}} \quad (1)
$$

$$
\epsilon_r l A_l R^{l-1} = -\frac{(l+1) B_l}{R^{l+2} } \quad (3)
$$

將第1式帶入第3式
$$
A_l = \frac{B_l}{R^{2l+1}}
$$

$$
\epsilon_r l \frac{B_l}{R^{2l+1}} R^{l-1} = -\frac{(l+1) B_l}{R^{l+2} }
$$

$$
\epsilon_r l \frac{B_l}{R^{l+2}} = -\frac{(l+1) B_l}{R^{l+2} }
$$

$$
\epsilon_r l = -(l+1)
$$

這很奇怪對吧? $\epsilon_r$ 隨 $l$ 而變? 這不合理。

問題在哪?問題在於我們把 $B_l$ 給消去，得出了不合理的結果。

只有一種可能，可以讓整件事合理化，那就是，$B_l=0, l\neq1$。

再根據，$A_l R^l = B_l R^{-(l+1)}$，$A_l=0, l\neq1$。

- 根據介電質球面兩側的邊界條件，當 $l = 1$

$$
A_1 R = -E_0 R + B_1 R^{-2} \quad (2)
$$

$$
\epsilon_r A_1 = -E_0 - 2 B_1 R^{-3} \quad (4)
$$

將(2)帶入(4)
$$
A_1 = -E_0 + B_1 R^{-3}
$$

$$
\epsilon_r( -E_0 + B_1 R^{-3}) = -E_0 - 2 B_1 R^{-3}
$$

$$
-\epsilon_rE_0 + \epsilon_rB_1 R^{-3} = -E_0 - 2 B_1 R^{-3}
$$

$$
\epsilon_rB_1 R^{-3} + 2 B_1 R^{-3} = \epsilon_rE_0 - E_0
$$

$$
B_1 = \frac{\epsilon_r - 1}{\epsilon_r + 2}R^{3}E_0
$$

將 $B_1$ 帶回(2)
$$
A_1 = -E_0 + \left( \frac{\epsilon_r - 1}{\epsilon_r + 2}R^{3}E_0 \right) R^{-3}
$$

$$
A_1 = -E_0 + \frac{\epsilon_r - 1}{\epsilon_r + 2}E_0
$$

$$
A_1 = \frac{-\epsilon_r - 2 + \epsilon_r - 1}{\epsilon_r + 2}E_0
$$

$$
A_1 = \frac{- 3}{\epsilon_r + 2}E_0
$$
