
$$
T_{ij} = \epsilon_0 \left( E_iE_j-\frac{1}{2}\delta_{ij}E^2 \right) +\frac{1}{\mu_0}\left( B_iB_j-\frac{1}{2}\delta_{ij}B^2 \right)
$$

---

$$
T_{xx} = \epsilon_0 \left( E_x^2-\frac{1}{2}E^2 \right)+\frac{1}{\mu_0}\left( B_x^2-\frac{1}{2}B^2 \right)
$$

$$
=\frac{\epsilon_0}{2}\left( E_x^2-E_y^2-E_z^2 \right)+\frac{1}{2\mu_0}\left( B_x^2-B_y^2-B_z^2 \right)
$$

$$
T_{xx} =\frac{\epsilon_0}{2}\left( E_x^2-E_y^2-E_z^2 \right)+\frac{1}{2\mu_0}\left( B_x^2-B_y^2-B_z^2 \right)
$$

$$
T_{yy} =\frac{\epsilon_0}{2}\left( E_y^2-E_x^2-E_z^2 \right)+\frac{1}{2\mu_0}\left( B_y^2-B_x^2-B_z^2 \right)
$$

$$
T_{zz} =\frac{\epsilon_0}{2}\left( E_z^2-E_x^2-E_y^2 \right)+\frac{1}{2\mu_0}\left( B_z^2-B_x^2-B_y^2 \right)
$$

$$
T_{xy} = \epsilon_0E_xE_y +\frac{1}{\mu_0}B_xB_y = T_{yx}
$$

$$
T_{xz} = \epsilon_0E_xE_z +\frac{1}{\mu_0}B_xB_z = T_{zx}
$$

$$
T_{yz} = \epsilon_0E_yE_z +\frac{1}{\mu_0}B_yB_z = T_{zy}
$$

---

$$
\left( \vec{a} \cdot \overleftrightarrow{T}\right)_j = \sum_{i=x,y,z} a_i\,T_{ij}
$$

$$
\left( \nabla \cdot \overleftrightarrow{T}\right)_j = \sum_{i=x,y,z} \nabla_i\,T_{ij} =\nabla_x\,T_{xj}+\nabla_y\,T_{yj}+\nabla_z\,T_{zj}
$$

---

$$
T_{xj} = \epsilon_0 \left( E_xE_j-\frac{1}{2}\delta_{xj}E^2 \right) + \frac{1}{\mu_0}\left( B_xB_j-\frac{1}{2}\delta_{xj}B^2 \right)
$$

$$
\nabla_x\,T_{xj} = \epsilon_0 \left( \nabla_x(E_xE_j)-\frac{1}{2}\delta_{xj}\nabla_xE^2 \right) + \frac{1}{\mu_0}\left( \nabla_x(B_xB_j)-\frac{1}{2}\delta_{xj}\nabla_xB^2 \right)
$$

$$
\nabla_x(E_xE_j) = \textcolor{blue}{\nabla_x(E_x)E_j}+E_x\nabla_x(E_j)
$$

$$
\nabla_x(B_xB_j) = \nabla_x(B_x)B_j+B_x\nabla_x(B_j)
$$

$$
\nabla_y\,T_{yj} = \epsilon_0 \left( \nabla_y(E_yE_j)-\frac{1}{2}\delta_{yj}\nabla_yE^2 \right) + \frac{1}{\mu_0}\left( \nabla_y(B_yB_j)-\frac{1}{2}\delta_{yj}\nabla_yB^2 \right)
$$

$$
\nabla_y(E_yE_j) = \textcolor{blue}{\nabla_y(E_y)E_j}+E_y\nabla_y(E_j)
$$

$$
\nabla_y(B_yB_j) = \nabla_y(B_y)B_j+B_y\nabla_y(B_j)
$$

$$
\nabla_z\,T_{zj} = \epsilon_0 \left( \nabla_z(E_zE_j)-\frac{1}{2}\delta_{zj}\nabla_zE^2 \right) + \frac{1}{\mu_0}\left( \nabla_z(B_zB_j)-\frac{1}{2}\delta_{zj}\nabla_zB^2 \right)
$$

$$
\nabla_z(E_zE_j) = \textcolor{blue}{\nabla_z(E_z)E_j}+E_z\nabla_z(E_j)
$$

$$
\nabla_z(B_zB_j) = \nabla_z(B_z)B_j+B_z\nabla_z(B_j)
$$

---

$$
\nabla_z(E_zE_j)+\nabla_z(E_zE_j)+\nabla_z(E_zE_j)
$$

$$
=\nabla_x(E_x)E_j+\nabla_y(E_y)E_j+\nabla_z(E_z)E_j
$$

$$
+E_x\nabla_x(E_j)+E_y\nabla_y(E_j)+E_z\nabla_z(E_j)
$$

$$
=\left( \nabla\cdot\vec{E} \right)E_j+\left( \vec{E} \cdot  \nabla \right)E_j
$$

$$
\delta_{xj}\nabla_xE^2+\delta_{yj}\nabla_yE^2+\delta_{zj}\nabla_zE^2
$$

$$
=\left( \delta_{xj}\nabla_x+\delta_{yj}\nabla_y+\delta_{zj}\nabla_z \right)E^2
$$

仔細檢視 $\delta_{xj}\nabla_x+\delta_{yj}\nabla_y+\delta_{zj}\nabla_z$
- 當 $j = x$ 時，$\delta_{xj} = 1, \delta_{yj} = 0, \delta_{zj} = 0$，所以該式變為 $\nabla_x$
- 當 $j = y$ 時，$\delta_{xj} = 0, \delta_{yj} = 1, \delta_{zj} = 0$，所以該式變為 $\nabla_y$
- 當 $j = z$ 時，$\delta_{xj} = 0, \delta_{yj} = 0, \delta_{zj} = 1$，所以該式變為 $\nabla_z$

因此，$\delta_{xj}\nabla_x+\delta_{yj}\nabla_y+\delta_{zj}\nabla_z = \nabla_j$

---

$$
\nabla_x\,T_{xj}+\nabla_y\,T_{yj}+\nabla_z\,T_{zj}
$$

$$
= \epsilon_0 \left[ \left( \nabla\cdot\vec{E} \right)E_j+\left( \vec{E} \cdot  \nabla \right)E_j-\frac{1}{2}\nabla_jE^2 \right]
$$

$$
+\frac{1}{\mu_0}\left[ \left( \nabla\cdot\vec{B} \right)B_j+\left( \vec{B} \cdot  \nabla \right)B_j-\frac{1}{2}\nabla_jB^2 \right]
$$

---

$$
\left( \nabla \cdot \overleftrightarrow{T}\right)_j = \sum_{i=x,y,z} \nabla_i\,T_{ij}
$$

$$
= \epsilon_0 \left[ \left( \nabla\cdot\vec{E} \right)E_j+\left( \vec{E} \cdot  \nabla \right)E_j\right]
$$

$$
+\frac{1}{\mu_0}\left[ \left( \nabla\cdot\vec{B} \right)B_j+\left( \vec{B} \cdot  \nabla \right)B_j\right]
$$

$$
-\nabla_j \left[ \frac{1}{2}\epsilon_0E^2 + \frac{1}{2\mu_0}B^2 \right]
$$

---

$$
\nabla \cdot \overleftrightarrow{T} 
$$

$$
= \epsilon_0 \left[ \left( \nabla\cdot\vec{E} \right)\vec{E}+\left( \vec{E} \cdot  \nabla \right)\vec{E}\right]
$$

$$
+\frac{1}{\mu_0}\left[ \left( \nabla\cdot\vec{B} \right)\vec{B}+\left( \vec{B} \cdot  \nabla \right)\vec{B}\right]
$$

$$
-\nabla \left[ \frac{1}{2}\epsilon_0E^2 + \frac{1}{2\mu_0}B^2 \right]
$$

---

### 量綱分析

$$
[\epsilon_0][電場]^2 = \frac{[電荷]}{[電場][面積]}\times[電場]^2
$$

$$
= \frac{[電荷][電場]}{[面積]} = \frac{[力]}{[面積]}
$$

$$
[1/\mu_0][磁場]^2 = \frac{[速度][電流]}{[電場][距離]}\times\frac{[電場]^2}{[速度]^2}
$$

$$
= \frac{[電流][電場]}{[距離][速度]} = \frac{[電流][電場][時間]}{[距離][距離]}
$$

$$
= \frac{[電荷][電場]}{[面積]} = \frac{[力]}{[面積]} 
$$


---

$$
[ \mu_0\epsilon_0\frac{\partial}{\partial t} S ]
$$

$$
= \frac{1}{[速度]^2[時間]}\times\frac{[功]}{[面積][時間]}
$$

$$
= \frac{[力][距離]}{[面積][距離]^2} = \frac{[力]}{[體積]}
$$

$$
[\nabla \cdot \overleftrightarrow{T} ]
$$

$$
=\frac{[動量]}{[體積][時間]} = \frac{[力]}{[體積]}
$$

